refactoring

MyOCL.thy
@@ -1,11 +1,12 @@
 theory MyOCL
-  imports Main ObjectModel MySQL
+  imports Main ObjectModel
 begin
 
 type_synonym var = string
 type_synonym ivar = string
 datatype att = AGE | EMAIL
 datatype as = LECTURERS | STUDENTS
+datatype entity = PERSON
 
 datatype OCLexp = Int nat 
   | Var var 
@@ -21,74 +22,7 @@ datatype OCLexp = Int nat
   | CollectPlus OCLexp OCLexp OCLexp 
   | PEAtt OCLexp
   | PEAs OCLexp "Enrollment list"
-  | AllInstances table
-
-fun transAtt :: "MyOCL.att \<Rightarrow> MySQL.col" where
-"transAtt MyOCL.AGE = MySQL.AGE" |
-"transAtt MyOCL.EMAIL = MySQL.EMAIL"
-
-fun transAs :: "MyOCL.as \<Rightarrow> MySQL.col" where
-"transAs MyOCL.STUDENTS = MySQL.STUDENTS" |
-"transAs MyOCL.LECTURERS = MySQL.LECTURERS"
-
-function (sequential) evalWithCtx :: "OCLexp \<Rightarrow> OCLexp \<Rightarrow> val \<Rightarrow> val" where
-"evalWithCtx (MyOCL.Int x) (MyOCL.IVar i) val = VInt x"
-(* For the time being *)
-| "evalWithCtx (MyOCL.Var x) (MyOCL.IVar i) val = (VObj x)" 
-| "evalWithCtx (MyOCL.IVar x) (MyOCL.IVar i) val = val"
-(* *)
-| "evalWithCtx (MyOCL.Eq e1 e2) (MyOCL.IVar i) val = 
-VBool (equalVal (evalWithCtx e1 (MyOCL.IVar i) val) (evalWithCtx e2 (MyOCL.IVar i) val))" 
-
-(*
-| "evalWithCtx (PEAtt (MyOCL.Att (Var v) MyOCL.AGE)) (MyOCL.IVar i) (VPerson p)
-= projVal (Col  MySQL.AGE ) (VObj v)"
-*)
-
-| "evalWithCtx (PEAs (MyOCL.As (IVar v)  MyOCL.STUDENTS) es) (MyOCL.IVar i) val
-= VList (extCol val  MySQL.STUDENTS es)"
-| "evalWithCtx (PEAs (MyOCL.As (IVar v)  MyOCL.LECTURERS) es) (MyOCL.IVar i) val
-= VList (extCol val  MySQL.LECTURERS es)"
-  by pat_completeness auto
-termination evalWithCtx
-  apply (relation  "(\<lambda>p. size (fst p)) <*mlex*> {}")
-  sorry
-
-(*  "(\<lambda>p. size (fst p)) <*mlex*> {}" *)
-(*
-
-| "evalWithCtx (PEAtt (MyOCL.Att (Var v) MyOCL.EMAIL)) (MyOCL.IVar i) val
-= projVal (Col  MySQL.EMAIL) (VObj v)"
-| "evalWithCtx (PEAs (MyOCL.As (Var v)  MyOCL.STUDENTS) es) (MyOCL.IVar i) val
-= VList (extCol (VObj v) MySQL.STUDENTS es)"
-| "evalWithCtx (PEAs (MyOCL.As (Var v)  MyOCL.LECTURERS) es) (MyOCL.IVar i) val
-= VList (extCol (VObj v) MySQL.LECTURERS es)"
-| "evalWithCtx (PEAtt (MyOCL.Att (IVar v)  MyOCL.AGE)) (MyOCL.IVar i) val
-= projVal (Col  MySQL.AGE) val"
-| "evalWithCtx (PEAtt (MyOCL.Att (IVar v)  MyOCL.EMAIL)) (MyOCL.IVar i) val
-= projVal (Col  MySQL.EMAIL) val"
-| "evalWithCtx (PEAs (MyOCL.As (IVar v)  MyOCL.STUDENTS) es) (MyOCL.IVar i) val
-= VList (extCol val  MySQL.STUDENTS es)"
-| "evalWithCtx (PEAs (MyOCL.As (IVar v)  MyOCL.LECTURERS) es) (MyOCL.IVar i) val
-= VList (extCol val  MySQL.LECTURERS es)"
-*)
-
-
-(*
-| "evalWithCtx (MyOCL.Size exp) var val
-= VList [VInt (sizeVal (evalWithCtx exp var val))]"
-| "evalWithCtx (MyOCL.IsEmpty exp) var val
-= VList [VBool (isEmptyVal (evalWithCtx exp var val))]"
-| "evalWithCtx (MyOCL.Exists src v body) var val
-= (evalWithCtx src var val)"
-*)
-
-fun filterWithBody :: "val list \<Rightarrow> OCLexp \<Rightarrow> OCLexp \<Rightarrow> val list" where
-"filterWithBody Nil var (exp) = Nil" 
-| "filterWithBody (Cons val vs) var exp = (if (isTrueVal (evalWithCtx exp var val)) 
-    then (val#(filterWithBody vs var exp))   
-    else filterWithBody vs var exp)"
-
+  | AllInstances entity
 
 fun partialEval :: "OCLexp \<Rightarrow> Objectmodel \<Rightarrow> OCLexp" where
 "partialEval (MyOCL.Int i) om = (MyOCL.Int i)"
@@ -100,29 +34,16 @@ fun partialEval :: "OCLexp \<Rightarrow> Objectmodel \<Rightarrow> OCLexp" where
 | "partialEval (MyOCL.As (Var v) as) om = (PEAs (MyOCL.As (Var v) as) (getEnrollmentList om))"
 | "partialEval (MyOCL.As (IVar v) as) om = (PEAs (MyOCL.As (IVar v) as) (getEnrollmentList om))"
 
-fun flatten :: "val list \<Rightarrow> val list" where
+fun flatten :: "val list list \<Rightarrow> val list" where
 "flatten [] = []" 
-| "flatten ((VList vs)#vss) = vs@(flatten vss)"
+| "flatten (v#vss) = v@(flatten vss)"
 
-fun collect :: "val list \<Rightarrow> OCLexp \<Rightarrow> OCLexp \<Rightarrow> val list" where
-"collect [] ivar exp = []"           
-| "collect (val#vs) ivar exp = (evalWithCtx exp ivar val)#(collect vs ivar exp)"
-
-fun eval :: "OCLexp \<Rightarrow> Objectmodel \<Rightarrow> val list" where
-"eval (MyOCL.Int i) om = [VInt i]"
-| "eval (MyOCL.Var x) om = [VObj x]"
-| "eval (MyOCL.Eq e1 e2) om = [VBool (equalValList (eval e1 om) (eval e2 om))]" 
-| "eval (MyOCL.Att (Var v) att) om = projValList (Col (transAtt att)) [VObj v]"
-| "eval (MyOCL.As (Var v) as) om = extCol (VObj v) (transAs as) (getEnrollmentList om)"
-| "eval (MyOCL.Size exp) om = [VInt (sizeValList (eval exp om))]"
-| "eval (MyOCL.IsEmpty exp) om = [VBool (isEmptyValList (eval exp om))]"
-| "eval (MyOCL.Exists src v body) om = [VBool (\<not> isEmptyValList (filterWithBody (eval src om) v (partialEval body om)))]"
-| "eval (MyOCL.AllInstances PERSON) om = mapPersonListToValList (getPersonList om)"
-| "eval (MyOCL.Collect src v body) om = collect (eval src om) v (partialEval body om)"
-| "eval (MyOCL.CollectPlus src v body) om = flatten (collect (eval src om) v (partialEval body om))"
-
-fun translate :: "OCLexp \<Rightarrow> MySQL.exp" where
-"translate (MyOCL.Int i) = MySQL.Int i" |
-"translate (Att (IVar p) att) = MySQL.Col (transAtt att)"
+(*
+fun collectAux :: "val list \<Rightarrow> OCLexp \<Rightarrow> Enrollment \<Rightarrow> val list" where
+"collectAux []  (As (IVar p) as.LECTURERS) en = []"
+| "collectAux (v#vs)  (As (IVar p) col) e = 
+(extCol v (transAs col) [e])
+@(collectAux vs  (As (IVar p) col) e)"
+*)
 
 end
