MyMain.thy
@@ -1,8 +1,6 @@
 theory MyMain
-  imports Main MyOCL MySQL
-begin
-
-(* PREVENT SLOW CHECKING... 
+  imports Main MyOCL MySQL OCLtoSQL
+  begin 
 
 (* self = caller \<equiv> SELECT self = caller *)
 lemma "eval (MyOCL.Eq (MyOCL.Var self) (MyOCL.Var caller)) om 
@@ -12,14 +10,12 @@ proof -
 qed     
 
 (* self.age = 30 \<equiv> SELECT age = 30 FROM Person WHERE id = self *)
-(*
 lemma "eval (MyOCL.Eq (MyOCL.Att (MyOCL.Var self) MyOCL.AGE) (MyOCL.Int 30)) om
 = exec (SelectFromWhere (MySQL.Eq (MySQL.Col (MySQL.AGE)) (MySQL.Int 30))
 (Table PERSON)
 (WHERE (MySQL.Eq (MySQL.Col (MySQL.ID)) (MySQL.Var self)))) om" 
   apply auto
   done        
-*)
 
 (* self.lecturers \<equiv> SELECT lecturers FROM Enrollment WHERE students = self *)
 lemma "eval (MyOCL.As (MyOCL.Var self) MyOCL.LECTURERS) om
@@ -140,9 +136,7 @@ case (Cons a list)
   then show ?thesis using filterWithBody_Person_noNeed_Ctx filterWithBody_Person by auto
   qed
   
-*)
 
-(*
 lemma collectPlus_on_Empty_Enrollment : "flatten (collect valList (IVar p) (PEAs (As (IVar p) as.LECTURERS) [])) = []"
 apply(induct valList)
 apply simp
@@ -150,18 +144,6 @@ apply auto
 done
 
 
-
-
-*)
- 
-lemma [simp]: "TEnrollment (OM [] es) = VNULL" 
-  sorry
-lemma [simp]: "TPerson (OM [] es) = VNULL" 
-  sorry
-lemma [simp]: "checkOnCondition VNULL VNULL exp = False " 
-  sorry
-lemma [simp]: "joinValListWithValList es [] exp = []"
-  sorry
 
 lemma [simp]: "joinValListWithValList (mapEnrollmentToValList es) ps exp =
                joinValListWithValList ps (mapEnrollmentToValList es) exp"
@@ -172,48 +154,41 @@ apply(induct xs)
 apply auto
 done
 
-lemma [simp]: "projVal (Col ID) a = a" 
-  sorry
-
 lemma [simp]: "projVal (Col col) (VEnrollment aa) =
                VPerson (getAssociationEnd col aa)"
-  sorry
+               sorry
 
-lemma [simp]: "projVal (Col col.LECTURERS) (VJoin [VPerson (getAssociationEnd col.STUDENTS aa), VEnrollment aa]) = 
-               projVal (Col col.LECTURERS) (VEnrollment aa)"
-  sorry
-
-(*
-lemma dist1 : "extCol a col (aa # es) = (extCol a col [aa]) @ (extCol a col es)"
-  sorry
-*)
-
-lemma lem0 : 
-      "extCol a col.LECTURERS es =
-       naselectList (joinValWithValList a (mapEnrollmentToValList es) (exp.Eq (Col col.STUDENTS) (Col ID))) (Col col.LECTURERS)"
- (*
- apply (induct es)
-   apply auto
-  done
-*)
-  sorry
-
-lemma lem1 : "flatten (collect ps (IVar p) (PEAs (As (IVar p) as.LECTURERS) es)) =
-               naselectList (joinValListWithValList (mapEnrollmentToValList es)  ps (exp.Eq (Col col.STUDENTS) (Col ID)))
-               (Col col.LECTURERS)"
-  sorry
-(*
-  apply (induct ps)
-   apply (simp)
-  apply (simp add: lem0)
-  done
-*)
 
 lemma [simp]: "collect (xs@ys) ivar exp = (collect xs ivar exp)@(collect ys ivar exp)"
 apply (induct xs)
 apply auto
-  done
+done
 
+
+(* ASSUMPTION *)       
+lemma [simp]: "collectPlus (mapPersonListToValList ps) (IVar p) (PEAs (As (IVar p) as.LECTURERS) (a # es))
+=  VPerson (getAssociationEnd col.LECTURERS a) # (collectPlus (mapPersonListToValList ps) (IVar p) (PEAs (As (IVar p) as.LECTURERS) es))"
+sorry
+
+
+(* FACT *)
+lemma [simp]:  "collectPlus src (IVar p) (PEAs (As (IVar p) as.LECTURERS) []) = []"
+sorry
+
+
+(* Person.allInstances()\<rightarrow>collect(p|p.lecturers)\<rightarrow>flatten()))
+\<equiv> SELECT lecturers FROM Enrollment *)
+lemma " eval (CollectPlus (AllInstances PERSON) (IVar p) (MyOCL.As (IVar p) (MyOCL.LECTURERS))) (OM ps es)
+= exec (SelectFrom (Col MySQL.LECTURERS) (Table ENROLLMENT)) (OM ps es)"
+apply auto
+apply (induct es)
+apply simp_all
+done
+
+(* ASSUMPTION *)
+lemma lem5 : "joinValWithValList (VEnrollment a) (mapPersonListToValList ps) (exp.Eq (Col col.LECTURERS) (Col ID))
+= [VJoin [VEnrollment a, (VPerson (getAssociationEnd col.LECTURERS a))]]"
+sorry
 
 (* Person.allInstances()\<rightarrow>collect(p|p.lecturers\<rightarrow>collect(l|l.email))
 \<equiv> SELECT email FROM Person JOIN Enrollment ON Person_id = lecturers *)
@@ -221,27 +196,11 @@ lemma "eval (Collect (CollectPlus (AllInstances PERSON) (IVar p) (MyOCL.As (IVar
 (IVar l) (MyOCL.Att (IVar l) (MyOCL.EMAIL))) (OM ps es)
 = exec (SelectFromJoin (Col MySQL.EMAIL) (Table ENROLLMENT) (JOIN (Table PERSON) (MySQL.Eq (Col MySQL.LECTURERS) (Col MySQL.ID)))) (OM ps es)"
 (* apply (simp add: TPerson_ValList TEnrollment_ValList) *)
-  apply (induct ps)
-  apply (simp)
-  apply (simp)
-
-
-(*
-OCL
- collect (naselectList (joinValWithValList (VPerson a) (mapEnrollmentToValList es) (exp.Eq (Col col.STUDENTS) (Col ID))) (Col col.LECTURERS))
-        (IVar l) (PEAtt (Att (IVar l) att.EMAIL)) =
-
-SQL
-naselectList (joinValWithValList (VPerson a) (mapEnrollmentToValList es) (exp.Eq (Col col.LECTURERS) (Col ID))) (Col col.EMAIL)
-*)
-
-   
-
-
+  apply (induct es)
+  apply (auto)
+  apply (simp add: lem5)
+  done
 
 
 end
-
-  (*exec (SelectFromJoin exp fromItem (JOIN fromItem2 onExp)) om*)
-
 
