OCLtoSQL.thy
@@ -1,0 +1,94 @@
+theory OCLtoSQL
+imports Main MySQL MyOCL
+begin
+
+fun transAtt :: "MyOCL.att \<Rightarrow> MySQL.col" where
+"transAtt MyOCL.AGE = MySQL.AGE" |
+"transAtt MyOCL.EMAIL = MySQL.EMAIL"
+
+fun transAs :: "MyOCL.as \<Rightarrow> MySQL.col" where
+"transAs MyOCL.STUDENTS = MySQL.STUDENTS" |
+"transAs MyOCL.LECTURERS = MySQL.LECTURERS"
+
+fun evalWithCtx :: "OCLexp \<Rightarrow> OCLexp \<Rightarrow> val \<Rightarrow> val" where
+"evalWithCtx (MyOCL.Int x) (MyOCL.IVar i) val = VInt x"
+(* For the time being *)
+| "evalWithCtx (MyOCL.Var x) (MyOCL.IVar i) val = (VObj x)" 
+(*| "evalWithCtx (MyOCL.IVar x) (MyOCL.IVar i) val = val"*)
+(* 
+| "evalWithCtx (MyOCL.Eq e1 e2) (MyOCL.IVar i) val = 
+VBool (equalVal (evalWithCtx e1 (MyOCL.IVar i) val) (evalWithCtx e2 (MyOCL.IVar i) val))" 
+*)
+| "evalWithCtx (PEAtt (MyOCL.Att (IVar v) MyOCL.EMAIL)) (MyOCL.IVar i) val
+= projVal (Col  MySQL.EMAIL) val"
+(*
+| "evalWithCtx (PEAs (MyOCL.As (IVar v)  MyOCL.STUDENTS) es) (MyOCL.IVar i) val
+= VList (extCol val  MySQL.STUDENTS es)"
+| "evalWithCtx (PEAs (MyOCL.As (IVar v)  MyOCL.LECTURERS) es) (MyOCL.IVar i) val
+= VList (extCol val  MySQL.LECTURERS es)"
+
+  by pat_completeness auto
+termination evalWithCtx
+  apply (relation  "(\<lambda>p. size (fst p)) <*mlex*> {}")
+  sorry
+*)
+
+(*  "(\<lambda>p. size (fst p)) <*mlex*> {}" *)
+(*
+
+| "evalWithCtx (PEAtt (MyOCL.Att (Var v) MyOCL.EMAIL)) (MyOCL.IVar i) val
+= projVal (Col  MySQL.EMAIL) (VObj v)"
+| "evalWithCtx (PEAs (MyOCL.As (Var v)  MyOCL.STUDENTS) es) (MyOCL.IVar i) val
+= VList (extCol (VObj v) MySQL.STUDENTS es)"
+| "evalWithCtx (PEAs (MyOCL.As (Var v)  MyOCL.LECTURERS) es) (MyOCL.IVar i) val
+= VList (extCol (VObj v) MySQL.LECTURERS es)"
+| "evalWithCtx (PEAtt (MyOCL.Att (IVar v)  MyOCL.AGE)) (MyOCL.IVar i) val
+= projVal (Col  MySQL.AGE) val"
+| "evalWithCtx (PEAtt (MyOCL.Att (IVar v)  MyOCL.EMAIL)) (MyOCL.IVar i) val
+= projVal (Col  MySQL.EMAIL) val"
+| "evalWithCtx (PEAs (MyOCL.As (IVar v)  MyOCL.STUDENTS) es) (MyOCL.IVar i) val
+= VList (extCol val  MySQL.STUDENTS es)"
+| "evalWithCtx (PEAs (MyOCL.As (IVar v)  MyOCL.LECTURERS) es) (MyOCL.IVar i) val
+= VList (extCol val  MySQL.LECTURERS es)"
+*)
+(*
+| "evalWithCtx (MyOCL.Size exp) var val
+= VList [VInt (sizeVal (evalWithCtx exp var val))]"
+| "evalWithCtx (MyOCL.IsEmpty exp) var val
+= VList [VBool (isEmptyVal (evalWithCtx exp var val))]"
+| "evalWithCtx (MyOCL.Exists src v body) var val
+= (evalWithCtx src var val)"
+*)
+
+fun filterWithBody :: "val list \<Rightarrow> OCLexp \<Rightarrow> OCLexp \<Rightarrow> val list" where
+"filterWithBody Nil var (exp) = Nil" 
+| "filterWithBody (Cons val vs) var exp = (if (isTrueVal (evalWithCtx exp var val)) 
+    then (val#(filterWithBody vs var exp))   
+    else filterWithBody vs var exp)"
+
+fun collect :: "val list \<Rightarrow> OCLexp \<Rightarrow> OCLexp \<Rightarrow> val list" where
+"collect [] ivar exp = []"           
+| "collect (val#vs) ivar exp = (evalWithCtx exp ivar val)#(collect vs ivar exp)"
+
+fun collectPlus :: "val list \<Rightarrow> OCLexp \<Rightarrow> OCLexp \<Rightarrow> val list" where
+"collectPlus [] ivar exp = []"           
+| "collectPlus (val#vs) ivar exp = (evalWithCtx exp ivar val)#(collectPlus vs ivar exp)"
+
+fun eval :: "OCLexp \<Rightarrow> Objectmodel \<Rightarrow> val list" where
+"eval (MyOCL.Int i) om = [VInt i]"
+| "eval (MyOCL.Var x) om = [VObj x]"
+| "eval (MyOCL.Eq e1 e2) om = [VBool (equalValList (eval e1 om) (eval e2 om))]" 
+| "eval (MyOCL.Att (Var v) att) om = projValList (Col (transAtt att)) [VObj v]"
+| "eval (MyOCL.As (Var v) as) om = extCol (VObj v) (transAs as) (getEnrollmentList om)"
+| "eval (MyOCL.Size exp) om = [VInt (sizeValList (eval exp om))]"
+| "eval (MyOCL.IsEmpty exp) om = [VBool (isEmptyValList (eval exp om))]"
+| "eval (MyOCL.Exists src v body) om = [VBool (\<not> isEmptyValList (filterWithBody (eval src om) v (partialEval body om)))]"
+| "eval (MyOCL.AllInstances PERSON) om = mapPersonListToValList (getPersonList om)"
+| "eval (MyOCL.Collect src v body) om = collect (eval src om) v (partialEval body om)"
+| "eval (MyOCL.CollectPlus src v body) om = collectPlus (eval src om) v (partialEval body om)"
+
+fun translate :: "OCLexp \<Rightarrow> MySQL.exp" where
+"translate (MyOCL.Int i) = MySQL.Int i" |
+"translate (Att (IVar p) att) = MySQL.Col (transAtt att)"
+
+end
